DER Integer2

code/ecdsap256/Hacl.Impl.P256.LowLevel.RawCmp.fst
@@ -34,10 +34,31 @@ let eq_0_u64 a = eq_u64_nCT a (u64 0)
 
 
 inline_for_extraction noextract
+val unsafe_bool_of_u8 (x: uint8 { v x == 0 \/ v x == pow2 8 - 1 }):
+  (b:bool { b <==> v x == 0 })
+
+let unsafe_bool_of_u8 x = 
+  match u8_to_UInt8 x with 
+  | 0uy -> true
+  | _ -> false
+
+
+inline_for_extraction noextract
 val unsafe_bool_of_u64 (x: uint64 { v x == 0 \/ v x == pow2 64 - 1 }):
   (b:bool { b <==> v x == 0 })
 
 let unsafe_bool_of_u64 x = 
   match u64_to_UInt64 x with 
   | 0UL -> true
+  | _ -> false
+
+
+inline_for_extraction noextract
+val unsafe_bool_of_u32 (x: uint32 { v x == 0 \/ v x == pow2 32 - 1 }):
+  (b:bool { b <==> v x == 0 })
+
+let unsafe_bool_of_u32 x = 
+  let open FStar.UInt32 in 
+  match u32_to_UInt32 x with 
+  |0ul  -> true
   | _ -> false
