code/ecdsap256/Hacl.Impl.ECDSA.DER.fst
@@ -1,0 +1,60 @@
+module Hacl.Impl.ECDSA.DER
+
+open FStar.HyperStack.All
+open FStar.HyperStack
+module ST = FStar.HyperStack.ST
+
+open Lib.IntTypes
+open Lib.Buffer
+
+open Hacl.Impl.P256.LowLevel.RawCmp
+open Lib.RawIntTypes
+
+let lenCoor = 32ul
+let integerIdentificator = 2 
+
+
+val decode: sigLen: size_t -> signature: lbuffer uint8 sigLen 
+  -> bufferForR: lbuffer uint8 lenCoor
+  -> bufferForS: lbuffer uint8 lenCoor -> 
+  Stack bool
+    (requires fun h -> live h signature /\ live h bufferForR /\ live h bufferForS)
+    (ensures fun h0 flag h1 -> 
+      let open Lib.Sequence in 
+
+      if v sigLen < 3 then flag = false else (
+      
+      let lengthIdentificator = index (as_seq h0 signature) 1 in 
+      let integerFirstIdentifier = index (as_seq h0 signature) 2 in 
+
+      if v sigLen >= 256 then flag = false else (* well *)
+      if v lengthIdentificator + 1 <> v sigLen then flag = false else 
+      if v integerFirstIdentifier = integerIdentificator then flag = false else True
+  
+  )
+)
+
+
+
+let decode sigLen signature bufferForR bufferS = 
+  if sigLen <. 3ul then false else
+  let zeroByte = index signature (size 0) in 
+  if unsafe_bool_of_u8 (neq_mask #U8 zeroByte (u8 30)) then false else
+  
+  let firstByte = index signature (size 1) in
+  if unsafe_bool_of_u8 (neq_mask #U8 firstByte (u8 255)) then false else begin
+    eq_mask_lemma firstByte (u8 255);
+  
+  let lengthFullSignature = to_u32 (incr firstByte) in 
+    incr_lemma firstByte;
+  let sizeAsUInt32 = size_to_uint32 sigLen in 
+    eq_mask_lemma lengthFullSignature sizeAsUInt32;
+  if unsafe_bool_of_u32 (eq_mask #U32 lengthFullSignature sizeAsUInt32) then false else
+  let secondByte = index signature (size 2) in 
+
+  if unsafe_bool_of_u8 (neq_mask #U8 secondByte (u8 integerIdentificator)) then false else 
+
+  
+
+    true
+  end
